Math/Relation/Segments.lean
@@ -1,0 +1,210 @@
+import Math.Relation.RelIso
+import Math.Data.Set.Basic
+
+open Relation
+
+structure InitialSegment (r: α -> α -> Prop) (s: β -> β -> Prop) extends r ↪r s where
+  isInitial: ∀a b, s b (toRelEmbedding a) -> b ∈ Set.range toRelEmbedding
+
+structure PrincipalSegment (r: α -> α -> Prop) (s: β -> β -> Prop) extends r ↪r s where
+  exists_top: ∃top: β, ∀b: β, s b top ↔ b ∈ Set.range toRelEmbedding
+
+infixl:25 " ≼i " => InitialSegment
+infixl:25 " ≺i " => PrincipalSegment
+
+variable {r: α -> α -> Prop} {s: β -> β -> Prop} {t: γ -> γ -> Prop}
+
+instance : FunLike (InitialSegment r s) α β where
+  coe f := f.toFun
+  coe_inj := by
+    intro ⟨_, _⟩ ⟨_, _⟩ eq
+    congr
+    exact DFunLike.coe_inj eq
+
+instance : FunLike (PrincipalSegment r s) α β where
+  coe f := f.toFun
+  coe_inj := by
+    intro ⟨_, _⟩ ⟨_, _⟩ eq
+    congr
+    exact DFunLike.coe_inj eq
+
+namespace InitialSegment
+
+def refl (r: α -> α -> Prop) : r ≼i r where
+  toRelEmbedding := RelEmbedding.refl
+  isInitial _ _ _ := Set.mem_range.mpr ⟨_, rfl⟩
+
+@[ext]
+def ext (a b: r ≼i s) : (∀x, a x = b x) -> a = b := DFunLike.ext a b
+
+def trans (h: r ≼i s) (g: s ≼i t): r ≼i t where
+  toRelEmbedding := RelEmbedding.trans h.toRelEmbedding g.toRelEmbedding
+  isInitial := by
+    intro a b t₀
+    have ⟨b₀, b_eq⟩ := Set.mem_range.mp <| g.isInitial _ _ t₀
+    subst b
+    have s₀ := g.resp_rel.mpr t₀
+    have ⟨a₀, a_eq⟩ := Set.mem_range.mp <| h.isInitial _ _ s₀
+    subst b₀
+    apply Set.mem_range.mpr
+    exact ⟨_, rfl⟩
+
+instance [IsTrichotomous s] [IsIrrefl s] [IsWellFounded r] : Subsingleton (r ≼i s) where
+  allEq := by
+    intro a b
+    ext x
+    induction x using (wellFounded r).induction with
+    | h x ih =>
+    apply extensional_of_trichotomous_of_irrefl s
+    intro y
+    apply Iff.intro
+    intro s₀
+    have ⟨y₀, eq⟩ := Set.mem_range.mp <| a.isInitial x y s₀
+    subst y
+    show s (a y₀) (b x)
+    rw [ih]
+    apply b.resp_rel.mp
+    apply a.resp_rel.mpr
+    assumption
+    apply a.resp_rel.mpr
+    assumption
+
+    intro s₀
+    have ⟨y₀, eq⟩ := Set.mem_range.mp <| b.isInitial x y s₀
+    subst y
+    show s (b y₀) (a x)
+    rw [←ih]
+    apply a.resp_rel.mp
+    apply b.resp_rel.mpr
+    assumption
+    apply b.resp_rel.mpr
+    assumption
+
+instance [IsWellOrder s] : Subsingleton (r ≼i s) :=
+  ⟨fun a => by let _ := a.toRelHom.wf; exact Subsingleton.elim a⟩
+
+def eq [IsWellOrder s] (f g : r ≼i s) (a) : f a = g a := by
+  rw [Subsingleton.elim f g]
+
+def antisymm_aux [IsWellOrder r] (f : r ≼i s) (g: s ≼i r) : Function.IsRightInverse f g :=
+  eq (f.trans g) (.refl _)
+
+def antisymm [IsWellOrder r] (f : r ≼i s) (g: s ≼i r) : r ≃r s where
+  toFun := f
+  invFun := g
+  leftInv := f.antisymm_aux g
+  rightInv :=
+    have := g.toRelEmbedding.wo
+    g.antisymm_aux f
+  resp_rel := f.resp_rel
+
+def eqv_or_principal [IsWellOrder s] (h: r ≼i s) :
+  Function.Surjective h ∨ ∃b, ∀x, s x b ↔ x ∈ Set.range h := by
+  apply Classical.or_iff_not_imp_right.mpr
+  intro g b
+  induction b using (wellFounded s).induction with
+  | h b ih =>
+  apply Classical.not_forall_not.mp
+  intro f
+  refine g ⟨b, ?_⟩
+  intro b'
+  apply Iff.intro
+  intro sb'b
+  apply Set.mem_range.mpr
+  obtain ⟨a, eq⟩ := ih b' sb'b
+  exact ⟨a, eq.symm⟩
+  intro mem
+  have ⟨a, eq⟩ := Set.mem_range.mp mem
+  subst b'
+  rcases trichotomous s (h a) b with ab | eq | ba
+  assumption
+  have := f _ eq
+  contradiction
+  have ⟨a', eq⟩ := Set.mem_range.mp <| h.isInitial _ _ ba
+  have := f _ eq.symm
+  contradiction
+
+def congr (eqr: r₀ ≃r r₁) (eqs: s₀ ≃r s₁) (g: r₀ ≼i s₀): r₁ ≼i s₁ where
+  toRelEmbedding := g.toRelEmbedding.congr eqr eqs
+  isInitial := by
+    intro a b  s'
+    rw [RelEmbedding.congr_apply] at s'
+    have : s₀ (eqs.symm b) (eqs.symm _) := eqs.symm.resp_rel.mp s'
+    rw [eqs.coe_symm] at this
+    have ⟨a', eq⟩ := Set.mem_range.mp <| g.isInitial _ _ this
+    apply Set.mem_range.mpr
+    exists eqr a'
+    rw [RelEmbedding.congr_apply]
+    rw [eqr.coe_symm, ←eq, eqs.symm_coe]
+
+end InitialSegment
+
+namespace PrincipalSegment
+
+theorem init [IsTrans s] (f : r ≺i s) (a : α) (b : β) (h : s b (f a)) : b ∈ Set.range f := by
+  obtain ⟨top, down⟩  := f.exists_top
+  apply (down _).mp
+  apply Relation.trans h
+  apply (down _).mpr
+  apply Set.mem_range'
+
+instance toPrincipal [IsTrans s] : Coe (r ≺i s) (r ≼i s) where
+  coe h := ⟨h.toRelEmbedding, h.init⟩
+
+def lt_of_lt_of_le (h: r ≺i s) (g: s ≼i t): r ≺i t where
+  toRelEmbedding := h.toRelEmbedding.trans g.toRelEmbedding
+  exists_top := by
+    obtain ⟨top, lt_top⟩ := h.exists_top
+    refine ⟨g top, ?_⟩
+    intro x
+    apply Iff.intro
+    intro tx
+    have ⟨x, eq⟩ := Set.mem_range.mp <| g.isInitial _ _ tx
+    subst eq
+    replace tx := g.resp_rel.mpr tx
+    have := (lt_top _).mp tx
+    apply Set.range_comp
+    assumption
+    intro mem
+    obtain ⟨x, eq⟩  := Set.mem_range.mp mem
+    subst eq
+    apply g.resp_rel.mp
+    apply (lt_top _).mpr
+    apply Set.mem_range'
+
+def congr (eqr: r₀ ≃r r₁) (eqs: s₀ ≃r s₁) (g: r₀ ≺i s₀): r₁ ≺i s₁ where
+  toRelEmbedding := g.toRelEmbedding.congr eqr eqs
+  exists_top := by
+    obtain ⟨top, lt_top⟩ := g.exists_top
+    exists eqs top
+    intro b
+    apply Iff.intro
+    intro h
+    have : s₀ (eqs.symm b) (eqs.symm (eqs top)) := eqs.symm.resp_rel.mp h
+    rw [eqs.coe_symm] at this
+    have := (lt_top _).mp this
+    have ⟨a', eq⟩ := Set.mem_range.mp this
+    apply Set.mem_range.mpr
+    exists eqr a'
+    rw [RelEmbedding.congr_apply, eqr.coe_symm, ←eq, eqs.symm_coe]
+    intro mem
+    have ⟨a', eq⟩ := Set.mem_range.mp mem
+    subst b
+    apply eqs.resp_rel.mp
+    apply (lt_top _).mpr
+    apply Set.mem_range'
+
+def trans [IsTrans t] (h: r ≺i s) (g: s ≺i t) : r ≺i t := lt_of_lt_of_le h g
+
+def coe_initial_seg_inj [IsTrans s] : Function.Injective (fun x: r ≺i s => (x: r ≼i s)) := by
+  intro x y eq
+  cases x; cases y
+  cases eq
+  congr
+
+instance [IsWellOrder s] : Subsingleton (r ≺i s) where
+  allEq a b := by
+    apply coe_initial_seg_inj
+    apply Subsingleton.allEq
+
+end PrincipalSegment
